@prefix rdfs: <http://www.w3.org/2000/01/rdf-schema#>.
@prefix rdf: <http://www.w3.org/1999/02/22-rdf-syntax-ns#>.
@prefix owl: <http://www.w3.org/2002/07/owl#>.
@prefix xsd: <http://www.w3.org/2001/XMLSchema#>.
@prefix hydra: <https://www.w3.org/ns/hydra/core#>.
@prefix void: <http://rdfs.org/ns/void#>.
@prefix vann: <http://purl.org/vocab/vann/>.
@prefix dct: <http://purl.org/dc/terms/>.
@prefix foaf: <http://xmlns.com/foaf/0.1/>.
@prefix sd: <http://www.w3.org/TR/sparql11-service-description/#>.
@prefix doap: <http://usefulinc.com/ns/doap#>.
@prefix oo: <http://linkedsoftwaredependencies.org/vocabularies/object-oriented#>.
@prefix om: <http://linkedsoftwaredependencies.org/vocabularies/object-mapping#>.

# ---------------------------------------- Metadata ----------------------------------------------

<http://linkedsoftwaredependencies.org/vocabularies/object-oriented#>
    a owl:Ontology;
    vann:preferredNamespacePrefix "oo";
    vann:preferredNamespaceUri "http://linkedsoftwaredependencies.org/vocabularies/object-oriented#";
    rdfs:label "Object-Oriented Components."@en;
    rdfs:comment "RDF vocabulary for describing Object-Oriented Components."@en;
    dct:title "Object-Oriented Components"@en;
    dct:issued "2017-04-08"^^xsd:date;
    dct:modified "2017-05-11"^^xsd:date;
    dct:creator <http://rubensworks.net/#me>.
<http://rubensworks.net/#me> foaf:name "Ruben Taelman".

# ------------------------------------------ Classes --------------------------------------------

oo:Module a rdfs:Class;
    rdfs:label "Module"@en;
    owl:sameAs doap:Version;
    rdfs:comment "A module can have several components"@en;
    rdfs:isDefinedBy <http://linkedsoftwaredependencies.org/vocabularies/object-oriented#>.

oo:Component a rdfs:Class;
    rdfs:label "Component"@en;
    rdfs:comment "A component is an instance or a class that can be instantiated based on parameters."@en;
    rdfs:subClassOf rdfs:Class;
    rdfs:isDefinedBy <http://linkedsoftwaredependencies.org/vocabularies/object-oriented#>.

oo:Class a rdfs:Class;
    rdfs:label "Class"@en;
    rdfs:comment "A class that can be instantiated based on parameters. All subtypes of classes are Instances."@en;
    rdfs:subClassOf oo:Component;
    rdfs:isDefinedBy <http://linkedsoftwaredependencies.org/vocabularies/object-oriented#>.

oo:AbstractClass a rdfs:Class;
    rdfs:label "Abstract Class"@en;
    rdfs:comment "An abstract class that can have subclasses that can be instantiated based on parameters."@en;
    rdfs:subClassOf oo:Class;
    rdfs:isDefinedBy <http://linkedsoftwaredependencies.org/vocabularies/object-oriented#>.

oo:Instance a rdfs:Class;
    rdfs:label "Instance"@en;
    rdfs:comment "An instance is an instantiation of a class."@en;
    rdfs:subClassOf oo:Component;
    rdfs:isDefinedBy <http://linkedsoftwaredependencies.org/vocabularies/object-oriented#>.

oo:Parameter a rdfs:Class;
    rdfs:label "Parameter"@en;
    rdfs:comment "Parameters are used to instantiate components."@en;
    rdfs:subClassOf rdfs:Property, om:ObjectMapping;
    rdfs:isDefinedBy <http://linkedsoftwaredependencies.org/vocabularies/object-oriented#>.

# ---------------------------------------- Properties --------------------------------------------

oo:component a rdf:Property;
    rdfs:label "has component"@en;
    rdfs:comment "Indicates that the subject module contains the object component that can be instantiated."@en;
    rdfs:isDefinedBy <http://linkedsoftwaredependencies.org/vocabularies/object-oriented#>;
    rdfs:domain oo:Module;
    rdfs:range oo:Component.

oo:parameter a rdf:Property;
    rdfs:label "has parameter"@en;
    rdfs:comment "The subject component has the object parameter that can be used in its configuration."@en;
    rdfs:isDefinedBy <http://linkedsoftwaredependencies.org/vocabularies/object-oriented#>;
    rdfs:subPropertyOf rdf:predicate;
    rdfs:domain oo:Class;
    rdfs:range oo:Parameter.

oo:arguments a rdf:Property;
    rdfs:label "has arguments"@en;
    rdfs:comment "The given function arguments must be mapped according to the given array mapping."@en;
    rdfs:isDefinedBy <http://linkedsoftwaredependencies.org/vocabularies/object-oriented#>;
    rdfs:domain oo:Class;
    rdfs:range om:ArrayMapping.

oo:constructorArguments a rdf:Property;
    rdfs:subPropertyOf oo:arguments;
    rdfs:label "has constructor arguments"@en;
    rdfs:comment "The parameter values of the given component's constructor must be mapped according to the given object mapper."@en;
    rdfs:isDefinedBy <http://linkedsoftwaredependencies.org/vocabularies/object-oriented#>.

oo:defaultValue a rdf:Property;
    rdfs:label "default value"@en;
    rdfs:comment "The default value of the parameter."@en;
    rdfs:isDefinedBy <http://linkedsoftwaredependencies.org/vocabularies/object-oriented#>;
    rdfs:domain oo:Parameter.

oo:uniqueValue a rdf:Property;
    rdfs:label "default value"@en;
    rdfs:comment "Indicate that the parameter can have at most one value."@en;
    rdfs:isDefinedBy <http://linkedsoftwaredependencies.org/vocabularies/object-oriented#>;
    rdfs:domain oo:Parameter;
    rdfs:range xsd:boolean.

oo:componentPath a rdf:Property;
    rdfs:label "class path"@en;
    rdfs:comment "The path to a component within a module."@en;
    rdfs:comment "Example value: 'my.package.name.Class'"@en;
    rdfs:isDefinedBy <http://linkedsoftwaredependencies.org/vocabularies/object-oriented#>;
    rdfs:domain oo:Component;
    rdfs:range xsd:string.
